reduction troubles

Reflection/Mutual.lean
@@ -1,8 +1,15 @@
--- Adaptation of https://dx.doi.org/10.4230/LIPIcs.FSCD.2020.23 for Lean4.
--- Agda source for the above lives at https://bitbucket.org/javra/inductive-families
+import Lean -- not essential: only for `Lean.Meta.getEqnsFor?` later
+
+/-
+  Adaptation of https://dx.doi.org/10.4230/LIPIcs.FSCD.2020.23 for Lean4.
+  Agda source for the above lives at https://bitbucket.org/javra/inductive-families
+-/
+
+set_option pp.proofs true
 
 -- # Syntax
 
+/-- Example for `Nat` is `U`, for `Vec` is `SPi Nat (fun n => U)`. -/
 inductive Tyₛ : Type 1
 | U : Tyₛ
 | SPi : (T : Type) -> (T -> Tyₛ) -> Tyₛ
@@ -23,7 +30,8 @@ inductive Varₛ : Conₛ -> Tyₛ -> Type 1
 open Varₛ
 
 set_option genInjectivity false in
-/-- `t : Tmₛ Γ A` corresponds to `Γ ⊢ t : A`. -/
+/-- `t : Tmₛ Γ A` corresponds to `Γ ⊢ t : A`.
+Original Agda: https://bitbucket.org/javra/inductive-families/src/717f404c220e17d0ac5917306fd74dd0c4883cde/agda/IF.agda#lines-25:27 -/
 inductive Tmₛ : Conₛ -> Tyₛ -> Type 1
 /-- A variable is a term.
 ```-
@@ -32,7 +40,7 @@ inductive Tmₛ : Conₛ -> Tyₛ -> Type 1
 Γ ⊢ₛ a : A
 ``` -/
 | var : Varₛ Γ A -> Tmₛ Γ A
-/-- Function application. Maybe problematic because `arg` is a black box.
+/-- Function application.
 ```-
 Γ ⊢ₛ f : (x : T) -> A x      arg : T
 -------------------------------------app-Intro
@@ -40,6 +48,9 @@ inductive Tmₛ : Conₛ -> Tyₛ -> Type 1
 ``` -/
 | app : Tmₛ Γ (SPi T A) -> (arg : T) -> Tmₛ Γ (A arg)
 infixl:50 " @ " => Tmₛ.app
+
+-- ! This fails:
+gen_injective_theorems% Tmₛ
 
 /-- Constructor types `... -> Self ...`.
 
@@ -94,13 +105,13 @@ section Examples
   def V_nil : Tyₚ Vₛ := El ((.var .vz) @ 0) -- Vec 0
 
   -- Vec : Nat -> U   ⊢ₛ   (n : Nat) -> A -> Vec n -> Vec (n + 1)
-  def V_cons (A : Type) : Tyₚ Vₛ :=
+  def V_cons {A : Type} : Tyₚ Vₛ :=
     PPi Nat fun n => -- (n : Nat) ->
       PPi A fun _ => -- A ->
         PFunc ((Tmₛ.var vz) @ n) <| -- Vec n ->
           El ((Tmₛ.var vz) @ (n + 1)) -- Vec (n + 1)
 
-  def V (A : Type) : Conₚ Vₛ := V_nil :: V_cons A :: []
+  def V (A : Type) : Conₚ Vₛ := V_nil :: @V_cons A :: []
 end Examples
 
 -- # Semantics
@@ -146,10 +157,25 @@ Vec 123
 The interesting thing here is that the quoted `"Vec"` is purely syntactic and doesn't use
 the actual `Vec` at all, it is merely a de-Brujin index into the context, which is entirely nameless.
 The purpose of `TmₛA` is to interpret the syntactic `"Vec 123"` into the actual `Vec 123`,
-by giving it the actual `Vec` interpretation via the `γₛ : ConₛA Γₛ`. -/
+by giving it the actual `Vec` interpretation via the `γₛ : ConₛA Γₛ`
+
+The [original Agda code](https://bitbucket.org/javra/inductive-families/src/717f404c220e17d0ac5917306fd74dd0c4883cde/agda/IFA.agda#lines-16:19)
+for `TmₛA` is the following, although it has `VarₛA` inlined, hence 3 cases:
+```agda
+_ᵃt : ∀{ℓ Γc B} → TmS Γc B → _ᵃc {ℓ} Γc → _ᵃS {ℓ} B
+(var vvz ᵃt)     (γ , α) = α
+(var (vvs t) ᵃt) (γ , α) = (var t ᵃt) γ
+((t $S α) ᵃt)    γ       = (t ᵃt) γ α
+```
+-/
 def TmₛA : {Γₛ : Conₛ} -> {Aₛ : Tyₛ} -> Tmₛ Γₛ Aₛ -> ConₛA Γₛ -> TyₛA Aₛ
 | Γ, A, @Tmₛ.var _   _ v  , γₛ => VarₛA v γₛ
 | Γ, _, @Tmₛ.app Γ T A t u, γₛ => (TmₛA t γₛ) u
+
+-- ! Why doesn't `by rfl` work for these two? Because of this I have to use casts in TmₛD which then spreads all over the place.
+@[simp] theorem TmₛA_var' : TmₛA (Tmₛ.var v) γₛ = VarₛA v γₛ := by rfl
+@[simp] theorem TmₛA_var  : TmₛA (Tmₛ.var v) γₛ = VarₛA v γₛ := by rw [TmₛA]
+@[simp] theorem TmₛA_app  : TmₛA (Tmₛ.app t u) γₛ = (TmₛA t γₛ) u := by rw [TmₛA]
 
 example {Vec : Nat -> Type} : @TmₛA (SPi Nat (fun _ => U) :: []) U ((.var .vz) @ 123) ⟨Vec, ⟨⟩⟩ = Vec 123 := rfl
 
@@ -172,7 +198,7 @@ example {Vec : Nat -> Type} {_A : Type}
   := rfl
 
 example {Vec : Nat -> Type} {A : Type}
-  : TyₚA (V_cons A) ⟨Vec, ⟨⟩⟩
+  : TyₚA (@V_cons A) ⟨Vec, ⟨⟩⟩
   = ((n : Nat) -> A -> Vec n -> Vec (n + 1))
   := rfl
 
@@ -195,3 +221,148 @@ example {Vec : Nat -> Type} {A : Type}
   : ConₚA (V A) ⟨Vec, ⟨⟩⟩
   = ((Vec 0) × ((n : Nat) -> A -> Vec n -> Vec (n + 1)) × Unit)
   := rfl
+
+-- ## Displayed Algebras
+
+/-- Compute motive type.
+
+Example: `TyₛD (SPi Nat (fun _ => U)) Vec` reduces to `(n : Nat) -> Vec n -> Type`. -/
+def TyₛD : (Aₛ : Tyₛ) -> TyₛA Aₛ -> Type 1
+| U, T => T -> Type
+| SPi T Aₛ, f => (t : T) -> TyₛD (Aₛ t) (f t)
+
+/-- Compute motive type for each mutually defined inductive type.
+
+Example:
+```
+ConₛD Vₛ ⟨Vec, ⟨⟩⟩
+```
+reduces to just one motive type:
+```
+((t : Nat) → Vec t -> Type) × Unit
+``` -/
+def ConₛD : (Γₛ : Conₛ) -> ConₛA Γₛ -> Type 1
+| .nil, _ => PUnit
+| .cons A Γ, ⟨a, γ⟩ => TyₛD A a × ConₛD Γ γ
+
+example {Vec : Nat -> Type} : ConₛD Vₛ ⟨Vec, ⟨⟩⟩ = (((t : Nat) → Vec t -> Type) × PUnit.{2}) := rfl
+
+def VarₛD : (v : Varₛ Γₛ Aₛ) -> ConₛD Γₛ γₛ -> TyₛD Aₛ (VarₛA v γₛ)
+| .vz  , ⟨a, _⟩ => a
+| .vs v, ⟨a, γD⟩ => VarₛD v γD
+
+/--
+The [original Agda code](https://bitbucket.org/javra/inductive-families/src/717f404c220e17d0ac5917306fd74dd0c4883cde/agda/IFD.agda#lines-17:20)
+for this is, again with `VarₛD` inlined:
+```agda
+ᵈt : ∀{ℓ' ℓ Γc B}(t : TmS Γc B){γc : _ᵃc {ℓ} Γc} → ᵈc {ℓ'} Γc γc → ᵈS {ℓ'} B ((t ᵃt) γc)
+ᵈt (var vvz)     (γcᵈ , αᵈ) = αᵈ
+ᵈt (var (vvs t)) (γcᵈ , αᵈ) = ᵈt (var t) γcᵈ
+ᵈt (t $S α)      γcᵈ        = ᵈt t γcᵈ α
+``` -/
+-- ! TmₛD needs casts because reduction behaviour of TmₛA is broken.
+def TmₛD : {Γₛ : Conₛ} -> {Aₛ : Tyₛ} -> {γₛ : ConₛA Γₛ} -> (t : Tmₛ  Γₛ Aₛ) -> ConₛD Γₛ γₛ -> TyₛD Aₛ (TmₛA t γₛ)
+| A :: Γₛ, _, γₛ, .var v                    , γD => TmₛA_var ▸ VarₛD v γD
+|      Γₛ, _, γₛ, .app (T := T) (A := A) t u, γD => TmₛA_app ▸ TmₛD t γD u
+
+#eval Lean.Meta.getEqnsFor? ``TmₛA -- Works just fine.
+#eval Lean.Meta.getEqnsFor? ``TmₛD -- ! TmₛD fails to generate equation theorems.
+
+-- Manually proving equation theorems (.var, then .app) for TmₛD:
+theorem TmₛD_var {v : Varₛ Γₛ Aₛ} {γₛD : ConₛD Γₛ γₛ} : TmₛD (Tmₛ.var v) γₛD = TmₛA_var ▸ VarₛD v γₛD := by
+  unfold TmₛD
+  cases Γₛ with
+  | nil => sorry -- I give up.
+  | cons => simp
+
+/-- Example:
+```
+@TyₚD Vₛ ⟨Vec A, ⟨⟩⟩ V_nil ⟨P, ⟨⟩⟩ Vec.nil
+  = P 0 Vec.nil
+```
+Example:
+```
+@TyₚD Vₛ ⟨Vec A, ⟨⟩⟩ V_cons ⟨P, ⟨⟩⟩ Vec.cons
+  = ((n : Nat) -> (a : A) -> (v : Vec A n) -> P n v -> P (n + 1) (Vec.cons n a v))
+``` -/
+-- Note: The `Self` here can be a little misleading, as it may be a nested type with different indices.
+def TyₚD : (A : Tyₚ Γₛ) -> ConₛD Γₛ γₛ -> TyₚA A γₛ -> Type
+| El         Self, γD, self => TmₛD Self γD self
+| PPi   T    Rest, γD, f    => (t : T) -> TyₚD (Rest t) γD (f t)
+| PFunc Self Rest, γD, f    => (self : TmₛA Self γₛ) -> TmₛD Self γD self -> TyₚD Rest γD (f self)
+
+inductive Vec (A : Type) : Nat -> Type
+| nil : Vec A 0
+| cons : (n : Nat) -> A -> Vec A n -> Vec A (n + 1)
+
+example {A : Type} {P : (n : Nat) -> Vec A n -> Type}
+  : @TyₚD Vₛ ⟨Vec A, ⟨⟩⟩ V_nil ⟨P, ⟨⟩⟩ Vec.nil
+  = P 0 Vec.nil
+  := rfl
+example {A : Type} {P : (n : Nat) -> Vec A n -> Type}
+  : @TyₚD Vₛ ⟨Vec A, ⟨⟩⟩ V_cons ⟨P, ⟨⟩⟩ Vec.cons
+  = ((n : Nat) -> (a : A) -> (v : Vec A n) -> P n v -> P (n + 1) (Vec.cons n a v))
+  := rfl
+
+/-- Example:
+```
+@ConₚD Vₛ ⟨Vec A, ⟨⟩⟩ (V_nil :: V_cons :: []) ⟨P, ⟨⟩⟩ ⟨Vec.nil, Vec.cons, ⟨⟩⟩
+```
+reduces to
+```
+  P 0 Vec.nil
+× ((n : Nat) -> (a : A) -> (v : Vec A n) -> P n v -> P (n + 1) (Vec.cons n a v))
+× PUnit
+``` -/
+def ConₚD : (Γ : Conₚ Γₛ) -> ConₛD Γₛ γₛ -> ConₚA Γ γₛ -> Type
+| .nil, _, _ => PUnit
+| .cons A Γ, γD, ⟨a, γ⟩ => TyₚD A γD a × ConₚD Γ γD γ
+
+example {P : (n : Nat) -> Vec A n -> Type}
+  : @ConₚD Vₛ ⟨Vec A, ⟨⟩⟩ (V_nil :: V_cons :: []) ⟨P, ⟨⟩⟩ ⟨Vec.nil, Vec.cons, ⟨⟩⟩
+  = (
+        (P 0 Vec.nil)
+      × ((n : Nat) -> (a : A) -> (v : Vec A n) -> P n v -> P (n + 1) (Vec.cons n a v))
+      × PUnit
+    )
+  := rfl
+
+-- ## Sections
+
+def TyₛS : (Aₛ : Tyₛ) -> (αₛ : TyₛA Aₛ) -> TyₛD Aₛ αₛ -> Type
+| U       , T , TD  => (t : T) -> TD t
+| SPi T Aₛ, fₛ, fₛd => (t : T) -> TyₛS (Aₛ t) (fₛ t) (fₛd t)
+
+def ConₛS : (Γₛ : Conₛ) -> (γₛ : ConₛA Γₛ) -> ConₛD Γₛ γₛ -> Type
+| .nil, ⟨⟩, ⟨⟩ => PUnit
+| .cons Aₛ Γₛ, ⟨αₛ, γₛ⟩, ⟨αₛd, γₛd⟩ => TyₛS Aₛ αₛ αₛd × ConₛS Γₛ γₛ γₛd
+
+def VarₛS : (x : Varₛ Γₛ Aₛ) -> ConₛS Γₛ γₛ γD -> TyₛS Aₛ (VarₛA x γₛ) (VarₛD x γD)
+| .vz  , ⟨αₛS, γₛS⟩ => αₛS
+| .vs v, ⟨ _, γₛS⟩ => VarₛS v γₛS
+
+theorem eq_cast_trans (h₁ : A = B) (h₂ : B = C) (x : A) : h₂ ▸ h₁ ▸ x = (h₂ ▸ h₁) ▸ x := by cases h₁; cases h₂; rfl -- https://leanprover.zulipchat.com/#narrow/stream/217875-Is-there-code-for-X.3F/topic/.28h.E2.82.82.20.E2.96.B8.20h.E2.82.81.29.20.E2.96.B8.20x.20.3D.20h.E2.82.82.20.E2.96.B8.20.28h.E2.82.81.20.E2.96.B8.20x.29/near/411362225 wow this URL
+@[simp] theorem eq_symm_cancel (T : B) (h : A = B) : h ▸ h.symm ▸ T = T := by rw [eq_cast_trans]
+
+-- set_option pp.notation false in
+def TmₛS  : {Γₛ : Conₛ} -> {Aₛ : Tyₛ} -> {γₛ : ConₛA Γₛ} -> {γₛD : ConₛD Γₛ γₛ} -> (t : Tmₛ  Γₛ Aₛ) -> ConₛS Γₛ γₛ γₛD -> TyₛS Aₛ (TmₛA t γₛ) (TmₛD t γₛD)
+| Γₛ, Aₛ, γₛ, γₛD, .var v, γₛS => by
+  have hA : TmₛA (Tmₛ.var v) γₛ  =            VarₛA v γₛ  := @TmₛA_var Γₛ Aₛ v γₛ
+  have hD : TmₛD (Tmₛ.var v) γₛD = hA.symm ▸ VarₛD v γₛD := by rw [TmₛD_var] -- this should work by rfl
+
+  -- Kyle's trick from a different thread: https://leanprover.zulipchat.com/#narrow/stream/270676-lean4/topic/rw.20term.20depended.20on.20by.20other.20argument/near/409268800
+  have {a b : TyₛA Aₛ} (hA : a = b) (d : TyₛD Aₛ a)
+    : TyₛS Aₛ a d
+    = TyₛS Aₛ b (hA ▸ d)
+    := by subst hA; rfl
+
+  rw [this hA (TmₛD (Tmₛ.var v) γₛD)]
+  rw [hD]
+  -- exact VarₛS v γₛS -- need to use eq_cast_trans here
+  sorry
+| _, _, _asdf, γD, .app (A := A) t u, γₛ => by
+  sorry
+
+def TyₚS  : (A : Tyₚ Γₛ) -> ConₛS Γₛ γₛ γD -> (α : TyₚA A γₛ) -> TyₚD A γD α -> Type := sorry
+
+def ConₚS : (Γ : Conₚ Γₛ) -> ConₛS Γₛ γₛ γD -> (γ : ConₚA Γ γₛ) -> ConₚD Γ γD γ -> Type := sorry
